@prefix swe:   <urn:x-gsml-rdf:types> .
@prefix iso19150-2: <http://def.isotc211.org/iso19150/-2/2012/base#> .
@prefix gsp:   <http://www.opengis.net/ont/geosparql#> .
@prefix rdf:   <http://www.w3.org/1999/02/22-rdf-syntax-ns#> .
@prefix owl:   <http://www.w3.org/2002/07/owl#> .
@prefix xsd:   <http://www.w3.org/2001/XMLSchema#> .
@prefix skos:  <http://www.w3.org/2004/02/skos/core#> .
@prefix gsmlv: <http://geosciml.org/ont/gsmlv#> .
@prefix rdfs:  <http://www.w3.org/2000/01/rdf-schema#> .
@prefix gsml:  <http://geosciml.org/ont/gsml#> .

gsml:positionalAccuracy
        a                owl:ObjectProperty ;
        rdfs:range       swe:Quantity ;
        skos:definition  "Quantitative values define the radius of an uncertainty buffer around a mappedFeature (eg: a positionAccuracy of 100 m for a line feature defines a buffer polygon of total width 200 m centred on the line).  Corresponds to ISO19115 DQ_PositionalAccuracy."@en .

gsml:samplingFrame  a    owl:ObjectProperty ;
        rdfs:range       skos:Concept ;
        skos:definition  "It is expected in GeoSciML that this byReference association will resolve to a SF_SpatialSamplingFeature instance which may include a spatial (GML) representation of the sampling frame (eg, a map tile, a 3D surface), or may resolve to a concept from a controlled source (eg,http://resource.geosciml.org/feature/cgi/EarthNaturalSurface)"@en .

gsml:GeologicFeature  a        owl:Class ;
        rdfs:subClassOf        [ a                  owl:Restriction ;
                                 owl:allValuesFrom  skos:Concept ;
                                 owl:onProperty     gsml:GeologicFeature.metadata
                               ] ;
        rdfs:subClassOf        [ a                  owl:Restriction ;
                                 owl:allValuesFrom  gsmlv:ControlledConcept ;
                                 owl:onProperty     gsml:classifier
                               ] ;
        rdfs:subClassOf        [ a                  owl:Restriction ;
                                 owl:allValuesFrom  gsml:GeologicFeature ;
                                 owl:onProperty     gsml:relatedFeature
                               ] ;
        rdfs:subClassOf        [ a                  owl:Restriction ;
                                 owl:allValuesFrom  gsml:MappedFeature ;
                                 owl:onProperty     gsml:occurrence
                               ] ;
        rdfs:subClassOf        [ a                  owl:Restriction ;
                                 owl:allValuesFrom  skos:Concept ;
                                 owl:onProperty     gsml:purpose
                               ] ;
        rdfs:subClassOf        [ a                  owl:Restriction ;
                                 owl:allValuesFrom  swe:Category ;
                                 owl:onProperty     gsml:GeologicFeature.observationMethod
                               ] ;
        iso19150-2:isAbstract  true ;
        skos:definition        "The abstract GeologicFeature class represents a conceptual feature that is hypothesized to exist coherently in the world.\r\n   * this corresponds with a \"legend item\" from a traditional geologic map\r\n   * while the bounding coordinates of a Geologic Feature may be described, its shape is not.\r\n\r\nThe implemented Geologic Feature instance acts as the \"description package\"\r\n\r\n    * the description package is classified according to its purpose as an Instance, TypicalNorm, or DefiningNorm."@en .

gsml:GeologicFeature.metadata
        a            owl:ObjectProperty ;
        rdfs:domain  gsml:GeologicFeature ;
        rdfs:range   skos:Concept .

gsml:classifier  a       owl:ObjectProperty ;
        rdfs:range       gsmlv:ControlledConcept ;
        skos:definition  "A standard description or definition of the feature type (eg; the definition of a particular Geologic Unit in a stratigraphic lexicon)"@en .

gsml:targetRole  a       owl:ObjectProperty ;
        rdfs:range       skos:Concept ;
        skos:definition  "The role played by the target geologic feature or object"@en .

gsml:GeologicRelation
        a                      owl:Class ;
        rdfs:subClassOf        [ a                  owl:Restriction ;
                                 owl:allValuesFrom  skos:Concept ;
                                 owl:onProperty     gsml:targetRole
                               ] ;
        rdfs:subClassOf        [ a                  owl:Restriction ;
                                 owl:allValuesFrom  skos:Concept ;
                                 owl:onProperty     gsml:sourceRole
                               ] ;
        rdfs:subClassOf        [ a                  owl:Restriction ;
                                 owl:allValuesFrom  skos:Concept ;
                                 owl:onProperty     gsml:relationship
                               ] ;
        iso19150-2:isAbstract  true ;
        skos:definition        "The GeologicRelation class is an abstract class that defines the general structure used to define relationships between any feature or object within GeoSciML. Relationships are always binary and directional.  There is always a single source and a single target.  The relationship is always defined from the perspective of the Source and is generally an active verb.\r\n\r\nExample:  a Source may point to an intrusive igneous rock body.  In this case, the Target would point to the appropriate host rock body and the relationship attribute would be 'intrudes'.  Other appropriate relationship attributes might include: overlies, offsets, crosscuts, folds, etc.\r\n\r\nMany other types of relationships can also be accommodated via GeologicRelation, for example, topological relations between spatial objects could be described where they are scientifically significant."@en .

gsml:GeologicFeature.observationMethod
        a                owl:ObjectProperty ;
        rdfs:domain      gsml:GeologicFeature ;
        rdfs:range       swe:Category ;
        skos:definition  "Feature ObservationMethod specifies the approach to acquiring the collection of attribute values that constitute an individual feature instance (e.g. point count, brunton compass on site, air photo interpretation,  field observation, hand specimen,  laboratory, aerial photography, creative imagination). ObservationMethod is a convenience property that provides a quick and dirty approach to observation metadata when data are reported using a feature view (as opposed to observation view). For a borehole, the GeologicFeature observation method specifies how the geologic properties were determined (eg, visual observation, or standard AzGS logging procedure (described in detail somewhere else)).  This property corresponds (loosely) to ISO19115 Lineage."@en .

gsml:MappedFeature.metadata
        a            owl:ObjectProperty ;
        rdfs:domain  gsml:MappedFeature ;
        rdfs:range   skos:Concept .

gsml:relationship  a     owl:ObjectProperty ;
        rdfs:range       skos:Concept ;
        skos:definition  "A term from a controlled vocabulary to describe the geologic relationship"@en .

gsml:relatedFeature  a   owl:ObjectProperty ;
        rdfs:range       gsml:GeologicFeature ;
        skos:definition  "Any geologic feature may be related to another geologic feature. For example, one geologic unit may \"overlie\" another geologic unit; a geologic unit may be \"intersected by\" a fault."@en .

<http://geosciml.org/ont/gsml>
        a                owl:Ontology ;
        owl:imports      <http://www.opengis.net/ont/geosparql> , <http://geosciml.org/ont/gsmlv> , <http://schemas.geosciml.org/rdf/types.ttl> ;
        owl:versionIRI   "http://geosciml.org/ont/gsml/3.2.0" ;
        owl:versionInfo  "3.2.0" ;
        skos:definition  "The GeoSciML-Core schema specifies a set of feature-types describing core geoscience information, including geologic units, structures, earth materials, relations between geologic features, and spatial geometries that represent geologic features on maps."@en .

gsml:MappedFeature  a    owl:Class ;
        rdfs:subClassOf  [ a                  owl:Restriction ;
                           owl:allValuesFrom  skos:Concept ;
                           owl:onProperty     gsml:MappedFeature.metadata
                         ] ;
        rdfs:subClassOf  [ a                  owl:Restriction ;
                           owl:allValuesFrom  gsml:GeologicFeature ;
                           owl:onProperty     gsml:specification
                         ] ;
        rdfs:subClassOf  [ a                  owl:Restriction ;
                           owl:allValuesFrom  gsp:Geometry ;
                           owl:onProperty     gsp:hasGeometry
                         ] ;
        rdfs:subClassOf  [ a                  owl:Restriction ;
                           owl:allValuesFrom  skos:Concept ;
                           owl:onProperty     gsml:samplingFrame
                         ] ;
        rdfs:subClassOf  [ a                  owl:Restriction ;
                           owl:allValuesFrom  skos:Concept ;
                           owl:onProperty     gsml:resolutionScale
                         ] ;
        rdfs:subClassOf  [ a                  owl:Restriction ;
                           owl:allValuesFrom  swe:Quantity ;
                           owl:onProperty     gsml:positionalAccuracy
                         ] ;
        rdfs:subClassOf  [ a                  owl:Restriction ;
                           owl:allValuesFrom  swe:Category ;
                           owl:onProperty     gsml:MappedFeature.observationMethod
                         ] ;
        skos:definition  "A MappedFeature is part of a geological interpretation. \r\nIt provides a link between a notional feature (description package) and one spatial representation of it, or part of it. (Exposures, Surface Traces and Intercepts, etc)\r\n    * the specific bounded occurrence, such as an outcrop or map polygon\r\n    * the Mapped Feature carries a geometry or shape\r\n          - the association with a Geologic Feature (legend item) provides specification of all the other descriptors\r\n          - the association with a Sampling Feature provides the context and dimensionality \r\n\r\nA Mapped Feature is always associated with some sampling feature - e.g. a mapping surface, a section, a Borehole (see BoreHolesAndObservation) etc. As noted on the diagram, if the associated sampling feature is a Borehole, then the shape associated with the MappedFeature will usually be either a point or an interval. This reconciles the 2-D (\"map\", section) and 1-D (borehole, traverse) viewpoints in a common abstraction."@en .

gsml:sourceRole  a       owl:ObjectProperty ;
        rdfs:range       skos:Concept ;
        skos:definition  "The role played by the source geologic feature or object"@en .

gsml:specification  a    owl:ObjectProperty ;
        rdfs:range       gsml:GeologicFeature ;
        skos:definition  "Point to the single geologic feature which describes the mapped feature."@en .

gsml:MappedFeature.observationMethod
        a                owl:ObjectProperty ;
        rdfs:domain      gsml:MappedFeature ;
        rdfs:range       swe:Category ;
        skos:definition  "MappedFeature ObservationMethod is a metadata snippet indicating how the spatial extent of the mapped feature was determined, and the basis for association of the geometry with some GeologicFeature specification to define a MappedFeature. For a borehole, the MappedInterval observation method indicates how the boundaries of the interval were defined (eg, linear measurement from borehole collar). ObservationMethod is a convenience property that provides a quick and dirty approach to observation metadata when data are reported using a feature view (as opposed to observation view). This property corresponds (loosely) to ISO19115 Lineage.  (eg: digitised, Global Positioning System, published map, fieldObservation, downhole survey, aerial photography, field survey)"@en .

gsml:occurrence  a       owl:ObjectProperty ;
        rdfs:range       gsml:MappedFeature ;
        skos:definition  "Points to any number of mapped features which are occurrences of the geologic feature.  Mapped features may all be from a single map or from several maps."@en .

gsml:GeologicFeatureRelation
        a                owl:Class ;
        rdfs:subClassOf  gsml:GeologicRelation ;
        skos:definition  "The GeologicFeatureRelation class is a concrete subtype of the abstract GeologicRelation class that is used to define relationships between geologic features, ie. structure-structure, unit-unit, and structure-unit relationships.\r\n\r\nRelationships are always binary and directional.  There is always a single source and a single target. The relationship is always defined from the perspective of the Source and is generally an active verb.\r\n\r\nExample:  a Source may point to an intrusive igneous rock body.  In this case, the Target would point to the appropriate host rock body and the relationship attribute would be 'intrudes'.  Other appropriate relationship attributes might include: overlies, offsets, crosscuts, folds, etc.\r\n\r\nTwo or more GeologicFeatures are associated in a GeologicFeatureRelation; each has a role in the relationship. Examples of geological roles include \"overlies\", \"is overlain by\", \"is younger\", \"is older\", \"intrudes\", \"is intruded by\", and so forth. In a relationship where an igneous unit intrudes a sedimentary unit, the geological relationship is \"intrudes\", the intruded sedimentary unit has the role \"host\", and the igneous unit has the role \"intrusion\"."@en .

gsml:resolutionScale  a  owl:ObjectProperty ;
        rdfs:range       skos:Concept ;
        skos:definition  "Reciprocal of equivalent scale of resolution for delineation of a feature's geometry. This is in contrast to positionAccuracy which is a measure of how well a feature is located relative to other features in the geographic reference system."@en .

gsml:purpose  a          owl:ObjectProperty ;
        rdfs:range       skos:Concept ;
        skos:definition  "Specification of the intended purpose/level of abstraction for a given feature or object instance. Scoped name because intention is asserted by author of the data instance. Values are: instance, typicalNorm, definingNorm."@en .
